Add `*` typing rule

theories/Values.v
@@ -4,32 +4,28 @@ From Lang Require Import
 
 Inductive Value : term -> Prop :=
   | ValAtom : forall id,
-      Value (TmAtom id O)
-  | ValPack : forall id arg ty curry ctx x,
+      Value (TmAtom id)
+  | ValPack : forall id arg arg_ty curry x ty,
+      let pack := TmPack id arg arg_ty curry in
+      let appl := TmAppl pack x in
       Value x ->
       Value curry ->
-      Typed ctx x ty ->
       AtomId id curry ->
-      Value (TmAppl (TmPack id arg ty curry) x)
-  | ValForA : forall arg ty body,
+      Typed [] appl ty ->
+      Value appl
+  | ValForA : forall arg arg_ty body ty,
+      let fora := TmForA arg arg_ty body in
       Value body -> (* Consider removing this *)
-      Value (TmForA arg ty body)
+      Typed [] fora ty ->
+      Value fora
   .
 
-(*
-TODO: Define on typing derivations, not terms.
-with Value : term -> Prop :=
-  | ValAtom : forall id,
-      (* NOTE:
-       * Must be at level 0: i.e. a term, not a type.
-       * In other words, if we want types to reduce,
-       * we have to decrement their level before evaluation.
-       *)
-      Value (TmAtom (AtomId id O))
-  | ValApAt : forall id,
-      Value (TmAppl (AtomAp arg_t arg_id etc)
-  | ValAtom : forall a,
-      ValueAtom a ->
-      Value (TmAtom a)
-  .
-*)
+Theorem values_always_typed : forall v,
+  Value v ->
+  exists ty, Typed [] v ty.
+Proof.
+  intros. induction H.
+  - exists (TmAtom id). constructor.
+  - exists ty. assumption.
+  - exists ty. assumption.
+Qed.
